DS/Okasaki_Ch10.v
@@ -51,7 +51,10 @@ match s with
     | One h t => Some (h, Zero t)
 end.
 
+(*
 Add Rec LoadPath "/home/Zeimer/Code/Coq".
+*)
+
 Require Import HSLib.Base.
 Require Import HSLib.Control.Functor.
 Require Import HSLib.Control.Monad.All.
